a b c d


Mesure terminale

Notons que : 
\begin{equation*}
dw^{i+1}\left( t\right) =dw^{N}\left( t\right) +\sum_{k=i+1}^{N-1}\left(
dw^{k}\left( t\right) -dw^{k+1}\left( t\right) \right)
\end{equation*}%
Donc : 
\begin{eqnarray*}
\frac{dL_{i}(t)}{L_{i}(t)} &=&\sigma _{i}(t)\cdot dw^{i+1}(t) \\
&=&\sigma _{i}(t)\cdot \left(
dw^{N}(t)+\sum_{k=i+1}^{N-1}(dw^{k}(t)-dw^{k+1}(t))\right) \\
&=&\sigma _{i}(t)\cdot dw^{N}(t)-\sum_{k=i+1}^{N-1}\frac{\delta
_{k}L_{k}\left( t\right) }{1+\delta _{k}L_{k}\left( t\right) }\,\sigma
_{i}\left( t\right) \cdot \sigma _{k}\left( t\right) dt
\end{eqnarray*}


